TCB/BinaryProps.v
@@ -4,7 +4,7 @@ Open Scope positive_scope.
 Open Scope N_scope.
 
 
-Lemma byte_to_N0: byte_to_N byte0 = 0.
+Lemma N_of_byte0: N_of_byte byte0 = 0.
 Proof.
   reflexivity.
 Qed.
@@ -21,18 +21,18 @@ Proof.
 Qed.
 
 Lemma word_of_word: forall w,
-  to_word (word_to_N w) = w.
+  to_word (N_of_word w) = w.
 Proof.
   destruct w as [b4 b3 b2 b1].
   unfold to_word.
   simpl. repeat rewrite fst_byte_of_byte.
-  unfold fst_byte, byte_to_N.
+  unfold fst_byte, N_of_byte.
   rewrite fst_four_bits_of_half_byte.
   destruct b4. simpl. destruct h; reflexivity.
 Qed.
 
 Definition word_and w1 w2 :=
-  to_word (N_and (word_to_N w1) (word_to_N w2)).
+  to_word (N_and (N_of_word w1) (N_of_word w2)).
 
 Lemma word_and_same w: word_and w w = w.
 Proof.
